CertifyingDatalog/TreeValidation.lean
@@ -1,0 +1,44 @@
+import CertifyingDatalog.Datalog
+import CertifyingDatalog.Unification
+
+
+variable {τ: signature} [DecidableEq τ.vars] [DecidableEq τ.constants] [DecidableEq τ.relationSymbols]
+
+def checkRuleMatch (P: List (rule τ)) (gr: groundRule τ): Bool :=
+  match P with
+  | List.nil => false
+  | List.cons hd tl =>
+    if Option.isSome (matchRule hd gr)
+    then true
+    else checkRuleMatch tl gr
+
+
+def treeValidatorHelper (P: List (rule τ)) (d: database τ) (t: proofTree τ): Bool :=
+  match t with
+  | proofTree.node a l =>
+    if l.isEmpty
+    then  if d.contains a
+          then true
+          else if checkRuleMatch P {head:= a, body := List.map root l}
+                then true
+                else false
+    else
+      if checkRuleMatch P {head:= a, body := List.map root l}
+      then List.all l.attach (fun ⟨x, _h⟩ => treeValidatorHelper P d x)
+      else false
+termination_by treeValidatorHelper P d t => sizeOf t
+decreasing_by
+  simp_wf
+  apply Nat.lt_trans (m:= sizeOf l)
+  apply List.sizeOf_lt_of_mem _h
+  simp
+
+
+def treeValidator (P: List (rule τ)) (d: database τ) (a: groundAtom τ)(t: proofTree τ): Bool :=
+  if root t = a
+  then treeValidatorHelper P d t
+  else false
+
+theorem treeValidatorIff (P: List (rule τ)) (d: database τ) (a: groundAtom τ)(t: proofTree τ): treeValidator P d a t = true ↔ isValid (List.toFinset P) d t ∧ root t = a :=
+by
+  sorry
